Coordination commit

backend/Mach_coop.v
@@ -13,6 +13,7 @@ Require Import Conventions.
 Require Stacklayout.
 
 Require Import Mach. 
+Require Import Stacking.
 
 Require Import mem_lemmas. (*for mem_forward*)
 Require Import core_semantics.
@@ -22,6 +23,13 @@ Definition genv := Genv.t fundef unit.
 
 Notation "a ## b" := (List.map a b) (at level 1).
 Notation "a # b <- c" := (Regmap.set b c a) (at level 1, b at next level).
+
+Inductive load_frame: Type :=
+| mk_load_frame:
+    forall (sp: block)       (**r pointer to argument frame *)
+           (args: list val)  (**r initial program arguments *)
+           (tys: list typ),  (**r initial argument types *)
+    load_frame.
 
 Section RELSEM.
 
@@ -35,123 +43,239 @@ Inductive Mach_core: Type :=
              (f: block)                (**r pointer to current function *)
              (sp: val)                 (**r stack pointer *)
              (c: code)                 (**r current program point *)
-             (rs: regset),             (**r register state *)
+             (rs: regset)              (**r register state *)
+             (loader: load_frame),     (**r program loader frame *)
       Mach_core
+
   | Mach_Callstate:
       forall (stack: list stackframe)  (**r call stack *)
              (f: block)                (**r pointer to function to call *)
-             (rs: regset),             (**r register state *)
+             (rs: regset)              (**r register state *)
+             (loader: load_frame),     (**r program loader frame *)
       Mach_core
 
-  (*Auxiliary state so that we can match to the coresemantics interface*)
-  | Mach_CallstateArgs: 
+  (*Auxiliary state: for marshalling arguments INTO memory*)
+  | Mach_CallstateIn: 
+      forall (f: block)                (**r pointer to function to call *)
+             (args: list val)          (**r arguments passed to initial_core *)
+             (tys: list typ),          (**r argument types *)
+      Mach_core
+
+  (*Auxiliary state: for marshalling arguments OUT OF memory*)
+  | Mach_CallstateOut: 
       forall (stack: list stackframe)  (**r call stack *)
-             (*(sp:val)                  stack pointer*)
-             (b: block)                (*global block holding the external function to be called*)
-             (f: external_function)    (**external function to be called *)
-             (vals: list val)          (**include explicit call arguments *)
-             (rs: regset),             (**r register state *)
+             (b: block)                (**r global block address of the external 
+                                            function to be called*)
+             (f: external_function)    (**r external function to be called *)
+             (vals: list val)          (**r at_external arguments *)
+             (rs: regset)              (**r register state *)
+             (loader: load_frame),     (**r program loader frame *)
       Mach_core
 
   | Mach_Returnstate:
       forall (stack: list stackframe)  (**r call stack *)
              (retty: option typ)       (**r optional return register int-floatness *)
-             (rs: regset),             (**r register state *)
+             (rs: regset)              (**r register state *)
+             (loader: load_frame),     (**r program loader frame *)
       Mach_core.
+
+(*NOTE [store_args] store_args is used to model program loading of
+  initial arguments.  Cf. NOTE [loader] below. *)
+
+Fixpoint store_args (sp: val) (ofs: Z) (args: list val) (tys: list typ) (m: mem) 
+         : option mem :=
+  match args,tys with
+    | nil,nil => Some m
+    | a::args',ty::tys' => 
+      match store_stack m sp ty (Int.repr (Stacklayout.fe_ofs_arg + 4*ofs)) a with
+        | None => None
+        | Some m' => store_args sp (ofs+1) args' tys' m'
+      end
+    | _,_ => None
+  end.
+
+Lemma store_stack_fwd m sp t i a m' :
+  store_stack m sp t i a = Some m' -> 
+  mem_forward m m'.
+Proof.
+unfold store_stack, Mem.storev.
+destruct (Val.add sp (Vint i)); try solve[inversion 1].
+apply store_forward.
+Qed.
+
+Lemma store_args_fwd sp ofs args tys m m' :
+  store_args sp ofs args tys m = Some m' -> 
+  mem_forward m m'.
+Proof.
+revert tys ofs m; induction args.
+simpl. destruct tys. intros ofs. inversion 1; subst. 
+solve[apply mem_forward_refl].
+intros ofs. solve[inversion 1].
+destruct tys. solve[inversion 1].
+inversion 1. revert H1.
+generalize
+  (Int.repr
+     match ofs with
+       | 0 => 0
+       | Z.pos y' => Z.pos y'~0~0
+       | Z.neg y' => Z.neg y'~0~0
+     end) as i; intro.
+case_eq (store_stack m sp t i a); [|solve[intros; congruence]].
+intros m0 H2 H3.
+apply store_stack_fwd in H2. 
+apply IHargs in H3.
+eapply mem_forward_trans; eauto.
+Qed.
+
+Lemma store_stack_unch_on stk z t i a m m' :
+  store_stack m (Vptr stk z) t i a = Some m' ->
+  Mem.unchanged_on (fun b ofs => b<>stk) m m'.
+Proof.
+unfold store_stack, Mem.storev. 
+case_eq (Val.add (Vptr stk z) (Vint i)); try solve[inversion 1].
+intros b i0 H H2. eapply Mem.store_unchanged_on in H2; eauto.
+intros i2 H3 H4. inv H. apply H4; auto.
+Qed.
+
+Lemma store_args_unch_on stk z ofs args tys m m' :
+  store_args (Vptr stk z) ofs args tys m = Some m' -> 
+  Mem.unchanged_on (fun b ofs => b<>stk) m m'.
+Proof.
+revert ofs tys m; induction args.
+simpl. destruct tys. inversion 1; subst. 
+  solve[apply Mem.unchanged_on_refl].
+solve[inversion 1].
+destruct tys. solve[inversion 1].
+inversion 1. revert H1.
+generalize (Int.repr
+             match ofs with
+               | 0 => 0
+               | Z.pos y' => Z.pos y'~0~0
+               | Z.neg y' => Z.neg y'~0~0
+             end) as ofs'. intros ofs'.
+case_eq (store_stack m (Vptr stk z) t ofs' a). 
+intros m2 H2 H3.
+eapply unchanged_on_trans with (m2 := m2); eauto.
+solve[eapply store_stack_unch_on; eauto].
+solve[apply store_stack_fwd in H2; auto].
+solve[inversion 2].
+Qed.
 
 Inductive mach_step: Mach_core -> mem -> Mach_core -> mem -> Prop :=
   | Mach_exec_Mlabel:
-      forall s f sp lbl c rs m,
-      mach_step (Mach_State s f sp (Mlabel lbl :: c) rs) m
-        (Mach_State s f sp c rs) m
+      forall s f sp lbl c rs m lf,
+      mach_step (Mach_State s f sp (Mlabel lbl :: c) rs lf) m
+                (Mach_State s f sp c rs lf) m
+
   | Mach_exec_Mgetstack:
-      forall s f sp ofs ty dst c rs m v,
+      forall s f sp ofs ty dst c rs m v lf,
       load_stack m sp ty ofs = Some v ->
-      mach_step (Mach_State s f sp (Mgetstack ofs ty dst :: c) rs) m
-        (Mach_State s f sp c (rs#dst <- v)) m
+      mach_step (Mach_State s f sp (Mgetstack ofs ty dst :: c) rs lf) m
+                (Mach_State s f sp c (rs#dst <- v) lf) m
+
   | Mach_exec_Msetstack:
-      forall s f sp src ofs ty c rs m m' rs',
+      forall s f sp src ofs ty c rs m m' rs' lf,
       store_stack m sp ty ofs (rs src) = Some m' ->
       rs' = undef_regs (destroyed_by_setstack ty) rs ->
-      mach_step (Mach_State s f sp (Msetstack src ofs ty :: c) rs) m
-        (Mach_State s f sp c rs') m'
+      mach_step (Mach_State s f sp (Msetstack src ofs ty :: c) rs lf) m
+                (Mach_State s f sp c rs' lf) m'
+
   | Mach_exec_Mgetparam:
-      forall s fb f sp ofs ty dst c rs m v rs',
+      forall s fb f sp ofs ty dst c rs m v rs' args0 tys0 sp0,
       Genv.find_funct_ptr ge fb = Some (Internal f) ->
       load_stack m sp Tint f.(fn_link_ofs) = Some (parent_sp s) ->
       load_stack m (parent_sp s) ty ofs = Some v ->
       rs' = (rs # temp_for_parent_frame <- Vundef # dst <- v) ->
-      mach_step (Mach_State s fb sp (Mgetparam ofs ty dst :: c) rs) m
-        (Mach_State s fb sp c rs') m
+      mach_step (Mach_State s fb sp (Mgetparam ofs ty dst :: c) rs (mk_load_frame args0 tys0 sp0)) m
+                (Mach_State s fb sp c rs' (...)) m
+
   | Mach_exec_Mop:
-      forall s f sp op args res c rs m v rs',
+      forall s f sp op args res c rs m v rs' lf,
       eval_operation ge sp op rs##args m = Some v ->
       rs' = ((undef_regs (destroyed_by_op op) rs)#res <- v) ->
-      mach_step (Mach_State s f sp (Mop op args res :: c) rs) m
-        (Mach_State s f sp c rs') m
+      mach_step (Mach_State s f sp (Mop op args res :: c) rs lf) m
+                (Mach_State s f sp c rs' lf) m
+
   | Mach_exec_Mload:
-      forall s f sp chunk addr args dst c rs m a v rs',
+      forall s f sp chunk addr args dst c rs m a v rs' lf,
       eval_addressing ge sp addr rs##args = Some a ->
       Mem.loadv chunk m a = Some v ->
       rs' = ((undef_regs (destroyed_by_load chunk addr) rs)#dst <- v) ->
-      mach_step (Mach_State s f sp (Mload chunk addr args dst :: c) rs) m
-        (Mach_State s f sp c rs') m
+      mach_step (Mach_State s f sp (Mload chunk addr args dst :: c) rs lf) m
+                (Mach_State s f sp c rs' lf) m
+
   | Mach_exec_Mstore:
-      forall s f sp chunk addr args src c rs m m' a rs',
+      forall s f sp chunk addr args src c rs m m' a rs' lf,
       eval_addressing ge sp addr rs##args = Some a ->
       Mem.storev chunk m a (rs src) = Some m' ->
       rs' = undef_regs (destroyed_by_store chunk addr) rs ->
-      mach_step (Mach_State s f sp (Mstore chunk addr args src :: c) rs) m
-        (Mach_State s f sp c rs') m'
+      mach_step (Mach_State s f sp (Mstore chunk addr args src :: c) rs lf) m
+                (Mach_State s f sp c rs' lf) m'
+
+  (*NOTE [loader]*)
+  | Mach_exec_Minitialize_call: 
+      forall m args tys m1 stk m2 fb,
+      Mem.alloc m 0 (4*Zlength args) = (m1, stk) ->
+      let sp := Vptr stk Int.zero in
+      store_args sp 0 args tys m1 = Some m2 -> 
+      mach_step (Mach_CallstateIn fb args tys) m
+        (Mach_Callstate nil fb (Regmap.init Vundef) (mk_load_frame stk args tys)) m2
+
   | Mach_exec_Mcall_internal:
-      forall s fb sp sig ros c rs m f f' ra callee,
+      forall s fb sp sig ros c rs m f f' ra callee lf,
       find_function_ptr ge ros rs = Some f' ->
       Genv.find_funct_ptr ge fb = Some (Internal f) ->
       return_address_offset f c ra ->
       (*NEW: check that the block f' actually contains a (internal) function:*)
-         Genv.find_funct_ptr ge f' = Some (Internal callee) ->
-      mach_step (Mach_State s fb sp (Mcall sig ros :: c) rs) m
-        (Mach_Callstate (Stackframe fb sp (Vptr fb ra) c :: s)
-                       f' rs) m
+      Genv.find_funct_ptr ge f' = Some (Internal callee) ->
+      mach_step (Mach_State s fb sp (Mcall sig ros :: c) rs lf) m
+                (Mach_Callstate (Stackframe fb sp (Vptr fb ra) c :: s) f' rs lf) m
+
   | Mach_exec_Mcall_external:
-      forall s fb sp sig ros c rs m f f' ra callee args,
+      forall s fb sp sig ros c rs m f f' ra callee args lf,
       find_function_ptr ge ros rs = Some f' ->
       Genv.find_funct_ptr ge fb = Some (Internal f) ->
       return_address_offset f c ra ->
-      (*NEW: check that the block f' actually contains a (external) function, and perform the "extra step":*)
-         Genv.find_funct_ptr ge f' = Some (External callee) ->
+      (*NEW: check that the block f' actually contains a (external)
+             function, and perform the "extra step":*)
+      Genv.find_funct_ptr ge f' = Some (External callee) ->
       extcall_arguments rs m sp (ef_sig callee) args ->
-      mach_step (Mach_State s fb sp (Mcall sig ros :: c) rs) m
-         (Mach_CallstateArgs (Stackframe fb sp (Vptr fb ra) c :: s) f' callee args rs) m
+      mach_step (Mach_State s fb sp (Mcall sig ros :: c) rs lf) m
+                (Mach_CallstateOut (Stackframe fb sp (Vptr fb ra) c :: s) 
+                  f' callee args rs lf) m
+
   | Mach_exec_Mtailcall_internal:
-      forall s fb stk soff sig ros c rs m f f' m' callee,
+      forall s fb stk soff sig ros c rs m f f' m' callee lf,
       find_function_ptr ge ros rs = Some f' ->
       Genv.find_funct_ptr ge fb = Some (Internal f) ->
       load_stack m (Vptr stk soff) Tint f.(fn_link_ofs) = Some (parent_sp s) ->
       load_stack m (Vptr stk soff) Tint f.(fn_retaddr_ofs) = Some (parent_ra s) ->
       Mem.free m stk 0 f.(fn_stacksize) = Some m' ->
       (*NEW: check that the block f' actually contains a function:*)
-         Genv.find_funct_ptr ge f' = Some (Internal callee) ->
-      mach_step (Mach_State s fb (Vptr stk soff) (Mtailcall sig ros :: c) rs) m
-        (Mach_Callstate s f' rs) m'
+      Genv.find_funct_ptr ge f' = Some (Internal callee) ->
+      mach_step (Mach_State s fb (Vptr stk soff) (Mtailcall sig ros :: c) rs lf) m
+                (Mach_Callstate s f' rs lf) m'
+
   | Mach_exec_Mtailcall_external:
-      forall s fb stk soff sig ros c rs m f f' m' callee args,
+      forall s fb stk soff sig ros c rs m f f' m' callee args lf,
       find_function_ptr ge ros rs = Some f' ->
       Genv.find_funct_ptr ge fb = Some (Internal f) ->
       load_stack m (Vptr stk soff) Tint f.(fn_link_ofs) = Some (parent_sp s) ->
       load_stack m (Vptr stk soff) Tint f.(fn_retaddr_ofs) = Some (parent_ra s) ->
       Mem.free m stk 0 f.(fn_stacksize) = Some m' ->
       (*NEW: check that the block f' actually contains a function:*)
-         Genv.find_funct_ptr ge f' = Some (External callee) ->
+      Genv.find_funct_ptr ge f' = Some (External callee) ->
       extcall_arguments rs m' (parent_sp s) (ef_sig callee) args ->
-      mach_step (Mach_State s fb (Vptr stk soff) (Mtailcall sig ros :: c) rs) m
-         (Mach_CallstateArgs s f' callee args rs) m'
+      mach_step (Mach_State s fb (Vptr stk soff) (Mtailcall sig ros :: c) rs lf) m
+                (Mach_CallstateOut s f' callee args rs lf) m'
+
   | Mach_exec_Mbuiltin:
-      forall s f sp rs m ef args res b t vl rs' m',
+      forall s f sp rs m ef args res b t vl rs' m' lf,
       external_call' ef ge rs##args m t vl m' ->
       rs' = set_regs res vl (undef_regs (destroyed_by_builtin ef) rs) ->
-      mach_step (Mach_State s f sp (Mbuiltin ef args res :: b) rs) m
-         (Mach_State s f sp b rs') m'
+      mach_step (Mach_State s f sp (Mbuiltin ef args res :: b) rs lf) m
+                (Mach_State s f sp b rs' lf) m'
+
 (*NO SUPPORT FOR ANNOT YET
   | Mach_exec_Mannot:
       forall s f sp rs m ef args b vargs t v m',
@@ -159,123 +283,96 @@ Inductive mach_step: Mach_core -> mem -> Mach_core -> mem -> Prop :=
       external_call' ef ge vargs m t v m' ->
       mach_step (Mach_State s f sp (Mannot ef args :: b) rs) m
          t (Mach_State s f sp b rs) m'*)
+
   | Mach_exec_Mgoto:
-      forall s fb f sp lbl c rs m c',
+      forall s fb f sp lbl c rs m c' lf,
       Genv.find_funct_ptr ge fb = Some (Internal f) ->
       find_label lbl f.(fn_code) = Some c' ->
-      mach_step (Mach_State s fb sp (Mgoto lbl :: c) rs) m
-        (Mach_State s fb sp c' rs) m
+      mach_step (Mach_State s fb sp (Mgoto lbl :: c) rs lf) m
+                (Mach_State s fb sp c' rs lf) m
+
   | Mach_exec_Mcond_true:
-      forall s fb f sp cond args lbl c rs m c' rs',
+      forall s fb f sp cond args lbl c rs m c' rs' lf,
       eval_condition cond rs##args m = Some true ->
       Genv.find_funct_ptr ge fb = Some (Internal f) ->
       find_label lbl f.(fn_code) = Some c' ->
       rs' = undef_regs (destroyed_by_cond cond) rs ->
-      mach_step (Mach_State s fb sp (Mcond cond args lbl :: c) rs) m
-        (Mach_State s fb sp c' rs') m
+      mach_step (Mach_State s fb sp (Mcond cond args lbl :: c) rs lf) m
+                (Mach_State s fb sp c' rs' lf) m
+
   | Mach_exec_Mcond_false:
-      forall s f sp cond args lbl c rs m rs',
+      forall s f sp cond args lbl c rs m rs' lf,
       eval_condition cond rs##args m = Some false ->
       rs' = undef_regs (destroyed_by_cond cond) rs ->
-      mach_step (Mach_State s f sp (Mcond cond args lbl :: c) rs) m
-        (Mach_State s f sp c rs') m
+      mach_step (Mach_State s f sp (Mcond cond args lbl :: c) rs lf) m
+                (Mach_State s f sp c rs' lf) m
+
   | Mach_exec_Mjumptable:
-      forall s fb f sp arg tbl c rs m n lbl c' rs',
+      forall s fb f sp arg tbl c rs m n lbl c' rs' lf,
       rs arg = Vint n ->
       list_nth_z tbl (Int.unsigned n) = Some lbl ->
       Genv.find_funct_ptr ge fb = Some (Internal f) ->
       find_label lbl f.(fn_code) = Some c' ->
       rs' = undef_regs destroyed_by_jumptable rs ->
-      mach_step (Mach_State s fb sp (Mjumptable arg tbl :: c) rs) m
-        (Mach_State s fb sp c' rs') m
+      mach_step (Mach_State s fb sp (Mjumptable arg tbl :: c) rs lf) m
+                (Mach_State s fb sp c' rs' lf) m
+
   | Mach_exec_Mreturn:
-      forall s fb stk soff c rs m f m',
+      forall s fb stk soff c rs m f m' lf,
       Genv.find_funct_ptr ge fb = Some (Internal f) ->
       load_stack m (Vptr stk soff) Tint f.(fn_link_ofs) = Some (parent_sp s) ->
       load_stack m (Vptr stk soff) Tint f.(fn_retaddr_ofs) = Some (parent_ra s) ->
       Mem.free m stk 0 f.(fn_stacksize) = Some m' ->
-      mach_step (Mach_State s fb (Vptr stk soff) (Mreturn :: c) rs) m
-        (Mach_Returnstate s (sig_res (fn_sig f)) rs) m'
+      mach_step (Mach_State s fb (Vptr stk soff) (Mreturn :: c) rs lf) m
+                (Mach_Returnstate s (sig_res (fn_sig f)) rs lf) m'
+
   | Mach_exec_function_internal:
-      forall s fb rs m f m1 m2 m3 stk rs',
+      forall s fb rs m f m1 m2 m3 stk rs' lf,
       Genv.find_funct_ptr ge fb = Some (Internal f) ->
       Mem.alloc m 0 f.(fn_stacksize) = (m1, stk) ->
       let sp := Vptr stk Int.zero in
       store_stack m1 sp Tint f.(fn_link_ofs) (parent_sp s) = Some m2 ->
       store_stack m2 sp Tint f.(fn_retaddr_ofs) (parent_ra s) = Some m3 ->
       rs' = undef_regs destroyed_at_function_entry rs ->
-      mach_step (Mach_Callstate s fb rs) m
-        (Mach_State s fb sp f.(fn_code) rs') m3
-(*auxiliary step that extracts call arguments and invoked external function,
-  in accordance with the core semantics interface
-  | Mach_exec_function_external:
-      forall s fb rs m ef args,
-      Genv.find_funct_ptr ge fb = Some (External ef) ->
-      extcall_arguments rs m (parent_sp s) (ef_sig ef) args ->
-      mach_step (Mach_Callstate s fb rs) m
-         (Mach_CallstateArgs s (*(parent_sp s)*) fb ef args rs) m*)
-(*NO RULE FOR EXTERNAL CALLS
-  | Mach_exec_function_external:
-      forall s fb rs m t rs' ef args res m',
-      Genv.fined_funct_ptr ge fb = Some (External ef) ->
-      extcall_arguments rs m (parent_sp s) (ef_sig ef) args ->
-      external_call' ef ge args m t res m' ->
-      rs' = set_regs (loc_result (ef_sig ef)) res rs ->
-      mach_step (Mach_Callstate s fb rs) m
-         t (Mach_Returnstate s rs') m'*)
+      mach_step (Mach_Callstate s fb rs lf) m
+                (Mach_State s fb sp f.(fn_code) rs' lf) m3
+
   | Mach_exec_return:
-      forall s f sp ra c retty rs m,
-      mach_step (Mach_Returnstate (Stackframe f sp ra c :: s) retty rs) m
-        (Mach_State s f sp c rs) m.
+      forall s f sp ra c retty rs m lf,
+      mach_step (Mach_Returnstate (Stackframe f sp ra c :: s) retty rs lf) m
+                (Mach_State s f sp c rs lf) m.
 
 End RELSEM.
 
-Definition Mach_initial_core (ge:genv) (v: val) (args:list val): 
-           option Mach_core :=match v with
-     | Vptr b i => 
-          if Int.eq_dec i Int.zero 
-          then match Genv.find_funct_ptr ge b with
-                 | None => None
-                 | Some f => 
-                    match f with Internal fi =>
-                     let tyl := sig_args (funsig f) in
-                     if val_has_type_list_func args (sig_args (funsig f))
-                        && vals_defined args
-                     then Some (Mach_Callstate
-                                      nil
-                                      b (Regmap.init Vundef)
-                                      (*TODO: Should be something like this: 
-                                       (Regmap.setlist
-                                          (reg??_arguments (funsig f)) 
-                                          args 
-                                          (Regmap.init Vundef)))*))
-                     else None
-                   | External _ => None
-                   end
+Definition Mach_initial_core (ge:genv) (v: val) (args:list val)
+           : option Mach_core := 
+  match v with
+    | Vptr b i => 
+      if Int.eq_dec i Int.zero 
+      then match Genv.find_funct_ptr ge b with
+             | None => None
+             | Some f => 
+               match f with 
+                 | Internal fi =>
+                   let tyl := sig_args (funsig f) in
+                   if val_has_type_list_func args (sig_args (funsig f))
+                      && vals_defined args
+                   then Some (Mach_CallstateIn b (encode_longs tyl args) tyl)
+                   else None
+                 | External _ => None
                end
-          else None
-     | _ => None
-    end.
-(*COMPCERT HAS THIS:
-Inductive initial_state (p: program): state -> Prop :=
-  | initial_state_intro: forall fb m0,
-      let ge := Genv.globalenv p in
-      Genv.init_mem p = Some m0 ->
-      Genv.find_symbol ge p.(prog_main) = Some fb ->
-      initial_state p (Callstate nil fb (Regmap.init Vundef) m0).
+           end
+      else None
+    | _ => None
+   end.
 
-Inductive final_state: state -> int -> Prop :=
-  | final_state_intro: forall rs m r retcode,
-      loc_result (mksignature nil (Some Tint)) = r :: nil ->
-      rs r = Vint retcode ->
-      final_state (Returnstate nil rs) m retcode.
-*)
+(*NOTE Halted when the stack contains just a single stack frame 
+  (modeling the program loader)*)
 
-(*Maybe generalize to other types?*)
 Definition Mach_halted (q : Mach_core): option val :=
     match q with 
       (*Return Tlong, which must be decoded*)
-      | Mach_Returnstate nil (Some Tlong) rs => 
+      | Mach_Returnstate nil (Some Tlong) rs lf => 
            match loc_result (mksignature nil (Some Tlong)) with
              | nil => None
              | r1 :: r2 :: nil => 
@@ -287,7 +384,7 @@ Definition Mach_halted (q : Mach_core): option val :=
            end
 
       (*Return a value of any other typ*)
-      | Mach_Returnstate nil (Some retty) rs => 
+      | Mach_Returnstate nil (Some retty) rs lf => 
            match loc_result (mksignature nil (Some retty)) with
             | nil => None
             | r :: TL => match TL with 
@@ -297,7 +394,7 @@ Definition Mach_halted (q : Mach_core): option val :=
            end
 
       (*Return Tvoid - modeled as integer return*)
-      | Mach_Returnstate nil None rs => Some (rs AX)
+      | Mach_Returnstate nil None rs lf => Some (rs AX)
 
       | _ => None
     end.
@@ -305,38 +402,26 @@ Definition Mach_halted (q : Mach_core): option val :=
 Definition Mach_at_external (c: Mach_core):
           option (external_function * signature * list val) :=
   match c with
-  | Mach_State _ _ _ _ _ => None
-  | Mach_Callstate _ _ _ => None
-  | Mach_CallstateArgs s (*sp*) fb ef args rs => 
-          Some (ef, ef_sig ef, decode_longs (sig_args (ef_sig ef)) args)
-(*
-  | Mach_CallstateArgs s (*sp*) fb args rs => 
-      match Genv.find_funct_ptr ge fb with
-        None => None
-      | Some (External ef) => Some (ef, ef_sig ef, decode_longs (sig_args (ef_sig ef)) args)
-      end*)
-(*  | Mach_CallstateArgs s (*sp*) ef args rs => 
-          Some (ef, ef_sig ef, decode_longs (sig_args (ef_sig ef)) args)*)
-  | Mach_Returnstate _ _ _ => None
+  | Mach_State _ _ _ _ _ _ => None
+  | Mach_Callstate _ _ _ _ => None
+  | Mach_CallstateIn _ _ _ => None
+  | Mach_CallstateOut s fb ef args rs lf => 
+      Some (ef, ef_sig ef, decode_longs (sig_args (ef_sig ef)) args)
+  | Mach_Returnstate _ _ _ _ => None
  end.
-(*CompCert:
-      Genv.find_funct_ptr ge fb = Some (External ef) ->
-      extcall_arguments rs m (parent_sp s) (ef_sig ef) args ->
-      external_call' ef ge args m t res m' ->
-      rs' = set_regs (loc_result (ef_sig ef)) res rs ->
-      mach_step (Callstate s fb rs) m
-         t (Mach_Returnstate s rs') m'*)
 
 Definition Mach_after_external (vret: option val)(c: Mach_core) : option Mach_core :=
   match c with 
-    Mach_CallstateArgs s (*sp*) fb ef args rs => 
+    Mach_CallstateOut s fb ef args rs lf => 
       match vret with
             | None => Some (Mach_Returnstate s (sig_res (ef_sig ef))
                              (set_regs (loc_result (ef_sig ef))
-                               (encode_long (sig_res (ef_sig ef)) Vundef) rs))
+                               (encode_long (sig_res (ef_sig ef)) Vundef) rs)
+                             lf)
             | Some v => Some (Mach_Returnstate s (sig_res (ef_sig ef))
                                (set_regs (loc_result (ef_sig ef))
-                                 (encode_long (sig_res (ef_sig ef)) v) rs))
+                                 (encode_long (sig_res (ef_sig ef)) v) rs)
+                               lf)
           end
   | _ => None
   end.
@@ -358,12 +443,12 @@ Variable return_address_offset: function -> code -> int -> Prop.
 Lemma Mach_corestep_not_at_external:
        forall ge m q m' q', mach_step return_address_offset ge q m q' m' -> 
               Mach_at_external q = None.
-  Proof. intros. inv H; try reflexivity. Qed.
+Proof. intros. inv H; try reflexivity. Qed.
 
 Lemma Mach_corestep_not_halted : forall ge m q m' q', 
        mach_step return_address_offset ge q m q' m' -> 
        Mach_halted q = None.
-  Proof. intros. inv H; reflexivity. Qed.
+Proof. intros. inv H; auto. Qed.
 
 Definition Mach_core_sem : CoreSemantics genv Mach_core mem.
   eapply (@Build_CoreSemantics _ _ _ 
@@ -376,9 +461,10 @@ Definition Mach_core_sem : CoreSemantics genv Mach_core mem.
     apply Mach_corestep_not_halted.
     apply Mach_at_external_halted_excl.
 Defined.
+
 End MACH_CORESEM.
 
-(************************NOW SHOW THAT WE ALSO HAVE A COOPSEM******)
+(******NOW SHOW THAT WE ALSO HAVE A COOPSEM******)
 
 Section MACH_COOPSEM.
 Variable return_address_offset: function -> code -> int -> Prop.
@@ -395,6 +481,10 @@ Lemma Mach_forward : forall g c m c' m'
    (*Mstore*)
      destruct a; simpl in H0; inv H0. 
      eapply store_forward. eassumption. 
+   (*initialize*)
+     eapply store_args_fwd in H0.
+     eapply mem_forward_trans; eauto.
+     solve[eapply alloc_forward; eauto].
    (*Mtailcall_internal*)
      eapply free_forward; eassumption.
    (*Mtailcall_external*)
